WIP

examples/lowparse/LowParse.Impl.Seq.fst
@@ -947,16 +947,28 @@ val seq_slice
     res == seq_slice_spec p b h lo hi 
   ))
 
-#set-options "--z3rlimit 16"
+#set-options "--z3rlimit 128"
 
 let seq_slice #b #t #p sv b lo hi =
   let h = HST.get () in
   let len1 = seq_offset_at sv b lo in
+  assert (len1 == seq_offset_at_spec p b h lo);
+  admit ()
+
+(*
+  assert (U32.v len1 == seq_offset_at_spec_nat p (S.as_seq h b) (U32.v lo));
   seq_offset_at_spec_nat_correct p (S.as_seq h b) (U32.v lo);
+  assert (Seq.length (S.as_seq h b) == U32.v (S.length b));
   let b1 = S.advance_slice b len1 in
+  let h1 = HST.get () in
+  assert (S.as_seq h1 b1 == S.as_seq h b1);
+  assert (Seq.length (S.as_seq h b1) == U32.v (S.length b1));
   let len2 = seq_offset_at sv b1 (U32.sub hi lo) in
+  assert (U32.v len2 == seq_offset_at_spec_nat p (S.as_seq h b1) (U32.v hi - U32.v lo));
   seq_offset_at_spec_nat_correct p (S.as_seq h b1) (U32.v hi - U32.v lo);
   let b2 = S.truncate_slice b1 len2 in
+  assert (b2 == seq_slice_spec p b h lo hi);
   b2
+*)
 
 #reset-options
